src/temporal_logic/pair.lean
@@ -7,8 +7,8 @@ open predicate
 
 section pair
 
-variables {α' : Type u} {β' : Type u₀} {γ' : Type u₁} {ω : Type u₂}
-variables (x : tvar α') (y : tvar β') (z : tvar γ')
+variables {α : Type u} {β : Type u₀} {γ : Type u₁} {ω : Type u₂}
+variables (x : tvar α) (y : tvar β) (z : tvar γ)
 
 @[tl_simp, simp]
 lemma pair_model (i : ℕ) :
@@ -16,31 +16,37 @@ i ⊨ ⦃x,y⦄ = (i ⊨ x,i ⊨ y) :=
 by { cases x, cases y, refl }
 
 @[reducible]
-def pair.fst : var (α' × β') α' :=
-⟨ @prod.fst α' β' ⟩
+def pair.fst : var (α × β) α :=
+⟨ @prod.fst α β ⟩
 
 @[reducible]
-def pair.snd : var (α' × β') β' :=
-⟨ @prod.snd α' β' ⟩
+def pair.snd : var (α × β) β :=
+⟨ @prod.snd α β ⟩
+
+abbreviation tvar.fst (p : var γ (α × β)) : var γ α :=
+pair.fst!p
+
+abbreviation tvar.snd (p : var γ (α × β)) : var γ β :=
+pair.snd!p
 
 @[tl_simp, simp]
-def pair.fst_mk (x : tvar α') (y : tvar β')
+def pair.fst_mk (x : tvar α) (y : tvar β)
 : pair.fst ! ⦃x,y⦄ = x :=
 by lifted_pred
 
 @[tl_simp, simp]
-def pair.fst_mk' (x : tvar α') (y : tvar β')
-: ⟨ @prod.fst α' β' ⟩ ! ⦃x,y⦄ = x :=
+def pair.fst_mk' (x : tvar α) (y : tvar β)
+: ⟨ @prod.fst α β ⟩ ! ⦃x,y⦄ = x :=
 pair.fst_mk _ _
 
 @[tl_simp, simp]
-def pair.snd_mk (x : tvar α') (y : tvar β')
+def pair.snd_mk (x : tvar α) (y : tvar β)
 : pair.snd ! ⦃x,y⦄ = y :=
 by lifted_pred
 
 @[tl_simp, simp]
-def pair.snd_mk' (x : tvar α') (y : tvar β')
-: ⟨ @prod.snd α' β' ⟩ ! ⦃x,y⦄ = y :=
+def pair.snd_mk' (x : tvar α) (y : tvar β)
+: ⟨ @prod.snd α β ⟩ ! ⦃x,y⦄ = y :=
 by lifted_pred
 
 @[tl_simp, simp]
@@ -53,29 +59,35 @@ def prod.map_right {α β γ} (f : β → γ) : α × β → α × γ
 open temporal.prod
 
 @[tl_simp, simp]
-lemma map_right_proj_pair (f : β' → γ')
+lemma map_right_proj_pair (f : β → γ)
 : ⟨map_right f⟩ ! ⦃x,y⦄ = ⦃x, ⟨f⟩ ! y⦄ :=
 by ext i ; simp [map_right] with tl_simp
 
 @[tl_simp, simp]
-lemma map_left_proj_pair (f : α' → γ')
+lemma map_left_proj_pair (f : α → γ)
 : ⟨map_left f⟩ ! ⦃x,y⦄ = ⦃⟨f⟩ ! x, y⦄ :=
 by ext i ; simp [map_left] with tl_simp
 
 @[tl_simp, simp]
-lemma map_proj_pair (f : α' → γ') (g : β' → ω)
+lemma map_proj_pair (f : α → γ) (g : β → ω)
 : ⟨prod.map f g⟩ ! ⦃x,y⦄ = ⦃⟨f⟩ ! x,⟨g⟩ ! y⦄ :=
 by ext i ; simp [prod.map] with tl_simp
 
 @[tl_simp, simp]
-lemma eta_pair (w : tvar (α' × β'))
-: ⦃pair.fst ! w, pair.snd ! w⦄ = w :=
+lemma eta_pair (w : tvar (α × β))
+: ⦃w.fst, w.snd⦄ = w :=
 by ext i ; simp [prod.map] with tl_simp
 
 @[tl_simp, simp]
-lemma next_pair (v₀ : tvar α') (v₁ : tvar β')
+lemma next_pair (v₀ : tvar α) (v₁ : tvar β)
 : ⊙⦃v₀,v₁⦄ = ⦃⊙v₀,⊙v₁⦄ :=
 by lifted_pred [next]
+
+@[tl_simp, simp, predicate]
+lemma to_fun_var_pair (f : tvar α → tvar β) (g : tvar α → tvar γ) (w : tvar α)
+: to_fun_var (λ w : tvar α, ⦃f w,g w⦄) w = ⦃to_fun_var f w,to_fun_var g w⦄ :=
+by { lifted_pred, simp! }
+
 end pair
 
 end temporal
