src/temporal_logic/spec.lean
@@ -7,27 +7,154 @@ namespace temporal
 
 open predicate fairness
 
-variables {α : Type u} {evt : Type u₀}
-variables (p : pred' α)
-variables (cs fs : evt → pred' α)
-variables (A : evt → act α)
+variables {α : Type u}
+
+structure mch' (evt : Type u₀) (α : Type u) :=
+  (init : pred' α)
+  (cs fs : evt → pred' α)
+  (A : option evt → act α)
+
+namespace mch'
+
+variable {evt : Type u₀}
+variables (m : mch' evt α)
+local notation `cs` := m.cs
+local notation `fs` := m.fs
+local notation `p` := m.init
+local notation `A` := m.A
+
+def effect : option evt → α → α → Prop
+ | none v v' := A none v v'
+ | (some e) v v' := v ⊨ cs e ∧ v ⊨ fs e ⋀ A (some e) v v'
+
+local notation `Next` := m.effect
+
+protected def event (e : evt) : event α :=
+⟨ cs e, fs e, A e ⟩
+
+def event' (aevt : Type u₀) (e : evt) (e' : aevt) : event (α × evt × aevt) :=
+⟨ cs e ! pair.fst
+, fs e ! pair.fst
+, λ ⟨s,ce,_⟩ ⟨s',_,ae'⟩, ae' = e' ∧ ce = e ∧ A e s s' ⟩
+
 
 @[simp, tl_simp]
 def spec_saf_spec (v : tvar α) (sch : tvar evt) : cpred :=
 p ! v ⋀
-◻(∃∃ e, sch ≃ ↑e ⋀ cs e ! v ⋀ fs e ! v ⋀ ⟦ v | A e ⟧)
+◻(∃∃ e, ⟦ v | m.effect e ⟧ )
 
 @[simp, tl_simp]
 def spec (v : tvar α) : cpred :=
 p ! v ⋀
-◻(∃∃ e, cs e ! v ⋀ fs e ! v ⋀ ⟦ v | A e ⟧) ⋀
+◻(∃∃ e, ⟦ v | m.effect e ⟧ ) ⋀
 ∀∀ e, sched (cs e ! v) (fs e ! v) ⟦ v | A e ⟧
 
 @[simp, tl_simp]
-def spec_sch (v : tvar α) (sch : tvar evt) : cpred :=
+def spec_sch (v : tvar α) (sch : tvar (option evt)) : cpred :=
 p ! v ⋀
-◻(∃∃ e, sch ≃ ↑e ⋀ cs e!v ⋀ fs e!v ⋀ ⟦ v | A e ⟧) ⋀
-∀∀ e, sched (cs e ! v) (fs e ! v) (sch ≃ e ⋀ ⟦ v | A e ⟧)
+◻(∃∃ e : option evt, sch ≃ ↑e ⋀ ⟦ v | m.effect e ⟧) ⋀
+∀∀ e : evt, sched (cs e ! v) (fs e ! v) (sch ≃ some e ⋀ ⟦ v | A ↑e ⟧)
 
+structure invariant (J : pred' α) : Prop :=
+  (init : p ⟹ J)
+  (step : ∀ e s s', Next e s s' → s ⊨ J → s' ⊨ J)
+
+end mch'
+
+structure mch (α : Type u) :=
+  {evt : Type u₀}
+  (init : pred' α)
+  (cs fs : evt → pred' α)
+  (A : option evt → act α)
+
+namespace mch
+variables (m : mch α)
+local notation `evt` := m.evt
+local notation `cs` := m.cs
+local notation `fs` := m.fs
+local notation `p` := m.init
+local notation `A` := m.A
+
+def effect : option evt → α → α → Prop
+ | none v v' := A none v v'
+ | (some e) v v' := v ⊨ cs e ∧ v ⊨ fs e ⋀ A (some e) v v'
+
+local notation `Next` := m.effect
+
+lemma act_of_effect {v v' : α} {e : option evt}
+  (h : Next e v v')
+: A e v v' :=
+by { cases e ; revert h ; simp [effect], }
+
+protected def event (e : evt) : event α :=
+⟨ cs e, fs e, A e ⟩
+
+def event' (aevt : Type u₀) (e : evt) (e' : aevt) : event (α × option evt × aevt) :=
+⟨ cs e ! pair.fst
+, fs e ! pair.fst
+, λ ⟨s,ce,_⟩ ⟨s',_,ae'⟩, ae' = e' ∧ ce = e ∧ A e s s' ⟩
+
+@[simp, tl_simp]
+def spec_saf_sch (v : tvar α) (sch : tvar (option evt)) : cpred :=
+p ! v ⋀
+◻(∃∃ e : option evt, sch ≃ ↑e ⋀ ⟦ v | m.effect e ⟧)
+
+@[simp, tl_simp]
+def spec (v : tvar α) : cpred :=
+p ! v ⋀
+◻(∃∃ e, ⟦ v | m.effect e ⟧ ) ⋀
+∀∀ e, sched (cs e ! v) (fs e ! v) ⟦ v | A e ⟧
+
+@[simp, tl_simp]
+def spec_sch (v : tvar α) (sch : tvar (option evt)) : cpred :=
+p ! v ⋀
+◻(∃∃ e : option evt, sch ≃ ↑e ⋀ ⟦ v | m.effect e ⟧) ⋀
+∀∀ e : evt, sched (cs e ! v) (fs e ! v) (sch ≃ some e ⋀ ⟦ v | A e ⟧)
+
+structure invariant (J : pred' α) : Prop :=
+  (init : p ⟹ J)
+  (step : ∀ e s s', Next e s s' → s ⊨ J → s' ⊨ J)
+
+variable {Γ : cpred}
+
+lemma spec_sch_of_spec_saf_sch (v : tvar α) (sch : tvar (option evt))
+  (h : Γ ⊢ m.spec_saf_sch v sch)
+  (h' : Γ ⊢ ∀∀ (e : m.evt), sched (m.cs e ! v) (m.fs e ! v) (sch ≃ ↑(some e) ⋀ ⟦ v | m.A (some e) ⟧))
+: Γ ⊢ m.spec_sch v sch :=
+begin [temporal]
+  simp at *,
+  split ; assumption,
+end
+
+lemma spec_of_spec_sch (v : tvar α) (sch : tvar (option evt))
+  (h : Γ ⊢ m.spec_sch v sch)
+: Γ ⊢ m.spec v :=
+begin [temporal]
+  simp at *,
+  revert h,
+  apply ctx_p_and_p_imp_p_and',
+  apply ctx_p_and_p_imp_p_and_right',
+  { monotonicity, apply p_exists_p_imp_p_exists,
+    simp, },
+  { apply p_forall_p_imp_p_forall,
+    intro, apply sched_imp_sched, simp },
+end
+
+lemma spec_of_spec_saf_sch (v : tvar α) (sch : tvar (option evt))
+  (h : Γ ⊢ m.spec_saf_sch v sch)
+  (h' : Γ ⊢ ∀∀ (e : m.evt), sched (m.cs e ! v) (m.fs e ! v) ⟦ v | m.A (some e) ⟧)
+: Γ ⊢ m.spec v :=
+begin [temporal]
+  simp at *,
+  split,
+  { revert h,
+    apply ctx_p_and_p_imp_p_and_right',
+    monotonicity,
+    apply p_exists_p_imp_p_exists,
+    simp  },
+  assumption,
+end
+
+end mch
 
 end temporal
